## Axiomatic probability

::: {#def-prob}
A *probability space* consists of $S$ and $P$, where $S$ is a sample
space, and $P$ is a function which takes an event $A\subseteq S$ as
input and returns $P(A)\in[0,1]$ such that

-   $P(\phi)=0$,
-   $P(S)=1$,
-   $P(\cup_{n=1}^{\infty}A_{n})=\sum_{n=1}^{\infty}P(A_{n})$ if
    $A_{1},A_{2},\ldots,A_{n}$ are disjoint.
:::

Note that this Definition does not imply any particular interpretation
of probability. In fact, any function $P$ that satisfies the axioms are
valid "probabilities". Thus, the theories of probability do not depend
on any particular interpretation. It is purely axiomatic. From the three
axioms, we can derive any property of probabilities. The interpretation
also matters, but it is more of a philosophical debate. 

:::{.callout-note}
## Two interpretations of probability

-   The *frequentist* view of probability is that it represents a
    long-run frequency over a large number of repetitions of an
    experiment: if we say a coin has probability 1/2 of Heads, that
    means the coin would land Heads 50% of the time if we tossed it over
    and over and over.
-   The *Bayesian* view of probability is that it represents a degree of
    belief about the event in question, so we can assign probabilities
    to hypotheses like "candidate A will win the election" or "the
    defendant is guilty" even if it isn't possible to repeat the same
    election or the same crime over and over again.
:::

::: {#prp-prob}
For any events $A$ and $B$, we have

-   $P(A^{c})=1-P(A)$
-   If $A\subseteq B$, then $P(A)\leq P(B).$
-   $P(A\cup B)=P(A)+P(B)-P(A\cap B)$.
:::

::: {.proof}
We prove the three properties by just using the Axioms. 

1) Since $A$ and $A^{c}$ are disjoint and their union is $S$, apply the
third axiom: $$P(S)=P(A\cup A^{c})=P(A)+P(A^{c});$$ By the second axiom,
$P(S)=1$. So $P(A)+P(A^{c})=1$.

2) The key is to break up the set into disjoint sets. If
$A\subseteq B$, then $B=A\cup(B\cap A^{c})$ where $A$ and $B\cap A^{c}$
are disjoint (draw a Venn diagram for intuition). By the third axiom, we
have $$P(B)=P(A\cup(B\cap A^{c}))=P(A)+P(B\cap A^{c})\geq P(A).$$

3) We can write $A\cup B$ as the union of the disjoint set $A$ and
$B\cap A^{c}$. Then by the third axiom,
$$P(A\cup B)=P(A\cup(B\cap A^{c}))=P(A)+P(B\cap A^{c}).$$
It suffices to show that $P(B\cap A^{c})=P(B)-P(A\cap B)$. Since
$B\cap A$ and $B\cap A^{c}$ are disjoint, we have
$$P(B)=P(B\cap A)+P(B\cap A^{c}).$$ So $P(B\cap A^{c})=P(B)-P(A\cap B)$
as desired.Â 
:::

The last property is a very useful formula for finding the probability
of a union of events when the events are not necessarily disjoint. 
We can generalize it to $n$ events.

::: {#thm-union}
For any events $A_{1},A_{2},\dots,A_{n}$, it holds that
$$\begin{aligned}
P(A_{1}\cup A_{2}\cdots\cup A_{n}) & =\sum_{j=1}^{n}P(A_{j})-\sum_{i<j}P(A_{i}\cap A_{j})+\sum_{i<j<k}P(A_{i}\cap A_{j}\cap A_{k})-\cdots\\
 & \quad(-1)^{n+1}P(A_{1}\cap\cdots\cap A_{n}).\end{aligned}$$
:::

This formula can be proved by induction using the axioms. Below is a
famous application (known as de Montmort's problem, named after French
mathematician Pierre Remond de Montmort) of the inclusion-exclusion
theorem.

::: {#exm-match}
(Matching problem) 
Suppose there are $n$ people who each check in a hat at a party. 
The hats are randomly returned to them without any concern for whose 
hat is whose. What is the probability that at least one person gets
their own hat back?
:::

::: solution
Let $A_j$ be the event: the $j$-th person gets his own hat. The problem 
is equivalent to find $P(A_{1}\cup A_{2}\cup\cdots\cup A_{n})$.

Since all position are equally likely, $P(A_{j})=\frac{1}{n}$. The
probability of there being two matches is:
$P(A_{1}\cap A_{2})=\frac{(n-2)!}{n!}=\frac{1}{n(n-1)}$. Similarly, the
probability of there being $k$ matches is:
$P(A_{1}\cap\cdots\cap A_{k})=\frac{(n-k)!}{n!}=\frac{1}{n(n-1)\cdots(n-k+1)}$.
Using the property of the union of events,
$$\begin{aligned}P(A_{1}\cup A_{2}\cup\cdots\cup A_{n})= & n\cdot\frac{1}{n}-\binom{n}{2}\frac{1}{n(n-1)}+\binom{n}{3}\frac{1}{n(n-1)(n-2)}-\cdots\\
= & 1-\frac{1}{2!}+\frac{1}{3!}-\frac{1}{4!}+\cdots+(-1)^{n+1}\frac{1}{n!}\\ \approx & 1-\frac{1}{e}.
\end{aligned}$$
:::

::: callout-tip
### Pattern matching with Taylor series
Pattern matching is a very useful technique. In the last step, we recognize that 
the Taylor series of $e^x$ is
$$e^x = 1 + x + \frac{x^2}{2!} +\frac{x^3}{3!}+\cdots $$
Therefore, $e^{-1} = 1 -1  + \frac{1}{2!} - \frac{1}{3!}+\cdots$
:::
